src/complexity.lean
@@ -1,0 +1,67 @@
+import degree
+
+variables {o_dom : Type*} {o_cod : Type*} [primcodable o_dom] [primcodable o_cod]
+
+structure admissible_numbering :=
+(numbering : ℕ → ℕ →. ℕ)
+(to_univ : ℕ → ℕ)
+(to_univ_computable : computable to_univ)
+(inv_univ : ℕ → ℕ)
+(inv_univ_computable : computable inv_univ)
+(numbering_to_univ : ∀ e, numbering e = ⟦to_univ e⟧⁰)
+(numbering_inv_univ : ∀ e, numbering (inv_univ e) = ⟦e⟧⁰)
+
+namespace admissible_numbering
+
+instance : has_coe_to_fun admissible_numbering (λ _, ℕ → ℕ →. ℕ) := ⟨numbering⟩
+
+def canonical : admissible_numbering :=
+{ numbering := univ0 ℕ ℕ,
+  to_univ := id,
+  to_univ_computable := computable.id,
+  inv_univ := id,
+  inv_univ_computable := computable.id,
+  numbering_to_univ := λ e, rfl,
+  numbering_inv_univ := λ e, rfl }
+
+variables {φ : admissible_numbering}
+open rcomputable rcomputable₂
+
+theorem exists_index {f : ℕ →. ℕ} :
+  partrec f ↔ ∃ e, φ e = f :=
+calc
+  partrec f ↔ f partrec_in (λ _, some 0 : ℕ →. ℕ) : ⟨λ h, h.to_rpart, λ h, rpartrec.le_part_part h (computable.const _)⟩
+        ... ↔ ∃ e, ⟦e⟧⁰ = f                       : rpartrec.exists_index
+        ... ↔ ∃ e, φ e = f
+  : ⟨by { rintros ⟨e, rfl⟩, refine ⟨φ.inv_univ e, φ.numbering_inv_univ _⟩ },
+     by { rintros ⟨e, rfl⟩, refine ⟨φ.to_univ e, eq.symm (φ.numbering_to_univ _)⟩ }⟩
+
+theorem recursion :
+  ∃ fixpoint : ℕ → ℕ, computable fixpoint ∧
+  ∀ {I : ℕ → ℕ} {i}, φ i = ↑ᵣI →
+    φ (fixpoint i) = φ (I (fixpoint i)) :=
+begin
+
+end
+
+theorem recursion {I : ℕ → ℕ} (h : computable I) :
+  ∃ n, φ n = φ (I n) :=
+begin
+
+end
+
+end admissible_numbering
+
+structure complexity_measure (φ : admissible_numbering) :=
+(measure : ℕ → ℕ →. ℕ)
+(convergence : ∀ e n, (φ e n).dom ↔ (measure e n).dom)
+(effective : computable_pred {n : ℕ × ℕ × ℕ | n.1 ∈ measure n.2.1 n.2.2})
+
+namespace complexity_measure 
+variables {φ : admissible_numbering} (Φ : complexity_measure φ)
+
+instance : has_coe_to_fun (complexity_measure φ) (λ _, ℕ → ℕ →. ℕ) := ⟨measure⟩
+
+
+
+end complexity_measure 
